Resolve sorry-proofs

Runtime/Network/Graph/Path/Subpaths.lean
@@ -9,26 +9,25 @@ def prefix? : Path graph start → Option (Path graph start)
   | cons _ nil => some nil
   | cons child subpath => subpath.prefix? >>= (cons child ·)
 
-theorem prefix?_iff_cons_prefix? {graph} {start : Class graph} {child : Class.Child start} {path₁ path₂ : Path graph child.class} :
-  (path₁.prefix? = some path₂) ↔ (cons child path₁).prefix? = some (cons child path₂) := by
-  constructor
-  all_goals
-    intro h
-    cases path₁
-    case nil => simp [prefix?] at h
-  case mp.cons => simp [prefix?, h]; rfl
-  case mpr.cons => sorry
-
-theorem prefix?_cons_eq_cons_prefix? {graph} {start : Class graph} {child : Class.Child start} {subpath subprefix : Path graph child.class} :
+theorem prefix?_cons_eq_cons_prefix?
+  {graph start} {child : Class.Child start} {subpath subprefix : Path graph child.class} :
   (subpath.prefix? = some subprefix) → (cons child subpath).prefix? = cons child subprefix := by
   intro h
   cases subpath
   case nil => simp [prefix?] at h
   case cons child' subpath => simp [prefix?, h]; rfl
 
-theorem prefix?_isSome_iff_isCons {path : Path graph start} : path.prefix?.isSome ↔ path.isCons := by
+theorem prefix?_isSome_iff_isCons {path : Path graph start} :
+  path.prefix?.isSome ↔ path.isCons := by
   constructor
-  case mp => sorry
+  case mp =>
+    intro h
+    induction path
+    case nil => simp [prefix?] at h
+    case cons child₁ subpath₁ hi =>
+      cases subpath₁
+      case nil => rfl
+      case cons child₂ subpath₂ => simp [isCons]
   case mpr =>
     intro h
     induction path
@@ -43,6 +42,23 @@ theorem prefix?_isSome_iff_isCons {path : Path graph start} : path.prefix?.isSom
         have ⟨subpath, hi⟩ := Option.isSome_iff_exists.mp hi
         simp [prefix?, hi, Option.isSome_iff_exists]
         exists .cons child₁ subpath
+
+theorem prefix?_iff_cons_prefix?
+  {graph start} {child : Class.Child start} {path₁ path₂ : Path graph child.class} :
+  (path₁.prefix? = some path₂) ↔ (cons child path₁).prefix? = some (cons child path₂) := by
+  constructor
+  all_goals
+    intro h
+    cases path₁
+    case nil => simp [prefix?] at h
+  case mp.cons => simp [prefix?, h]; rfl
+  case mpr.cons child subpath =>
+    have hs := prefix?_isSome_iff_isCons.mpr (@isCons_of_cons _ _ child subpath)
+    have ⟨_, hs⟩ := Option.isSome_iff_exists.mp hs
+    simp [hs, prefix?] at h ⊢
+    injection h with h
+    injection h
+    assumption
 
 def snd (path : Path graph start) (_ : path.isCons) : Class.Child start :=
   match path with
@@ -66,7 +82,8 @@ theorem suffix_class {path : Path graph start} {h} : (path.suffix h).class = pat
   case _ h => simp [isCons] at h
   · simp
 
-def split (path : Path graph start) (_ : path.isCons) : Σ «prefix» : Path graph start, Class.Child prefix.class :=
+def split (path : Path graph start) (_ : path.isCons) :
+  Σ «prefix» : Path graph start, Class.Child prefix.class :=
   match path with
   | nil => by contradiction
   | cons child nil => ⟨nil, child⟩
@@ -74,7 +91,8 @@ def split (path : Path graph start) (_ : path.isCons) : Σ «prefix» : Path gra
     let ⟨sub, cls⟩ := subpath.split (by simp_all [isCons_of_cons])
     ⟨cons child sub, cls⟩
 
-theorem split_class {path : Path graph start} (h : path.isCons) : (path.split h).snd.class = path.class := by
+theorem split_class {path : Path graph start} (h : path.isCons) :
+  (path.split h).snd.class = path.class := by
   induction path
   case nil => contradiction
   case cons child subpath hi =>
